src/model/Cell.v
@@ -491,118 +491,221 @@ Module Cell.
   Qed.
 
 
+  (* maximal & minimal messages satisfying a property *)
+
+  Lemma max_exists_aux P l:
+    (<<NONE: forall ts (IN: List.In ts l), ~ P ts>>) \/
+    exists max,
+      (<<SAT: P max>>) /\
+      (<<MAX: forall ts (IN: List.In ts l) (SAT: P ts),
+          Time.le ts max>>).
+  Proof.
+    induction l; auto. des; subst.
+    - destruct (classic (P a)).
+      + right. esplits; eauto.
+        i. inv IN; try refl.
+        exploit NONE; eauto. ss.
+      + left. ii. inv IN; ss.
+        exploit NONE; eauto.
+    - right. destruct (classic (P a)).
+      + destruct (TimeFacts.le_lt_dec a max).
+        * exists max. splits; ss.
+          i. des; subst; eauto.
+        * exists a. splits; ss.
+          i. des; subst; try refl.
+          exploit MAX; eauto. i.
+          etrans; eauto. econs. ss.
+      + esplits; eauto. i. inv IN; eauto. ss.
+  Qed.
+
+  Lemma max_exists P cell:
+    (<<NONE: forall from to msg
+                    (GET: get to cell = Some (from, msg)),
+        ~ P to>>) \/
+    exists from_max to_max msg_max,
+      (<<GET: get to_max cell = Some (from_max, msg_max)>>) /\
+      (<<SAT: P to_max>>) /\
+      (<<MAX: forall from to msg
+                     (GET: get to cell = Some (from, msg))
+                     (SAT: P to),
+          Time.le to to_max>>).
+  Proof.
+    specialize (finite cell). i. des.
+    specialize (max_exists_aux
+                  (fun ts => P ts /\
+                             exists from msg,
+                               get ts cell = Some (from, msg))
+                  dom).
+    i. des.
+    - left. ii. exploit H; eauto. i.
+      exploit NONE; eauto.
+    - right. esplits; eauto. i.
+      exploit H; eauto.
+  Qed.
+
+  Lemma min_exists_aux P l:
+    (<<NONE: forall ts (IN: List.In ts l), ~ P ts>>) \/
+    exists min,
+      (<<SAT: P min>>) /\
+      (<<MIN: forall ts (IN: List.In ts l) (SAT: P ts),
+          Time.le min ts>>).
+  Proof.
+    induction l; auto. des; subst.
+    - destruct (classic (P a)).
+      + right. esplits; eauto.
+        i. inv IN; try refl.
+        exploit NONE; eauto. ss.
+      + left. ii. inv IN; ss.
+        exploit NONE; eauto.
+    - right. destruct (classic (P a)).
+      + destruct (TimeFacts.le_lt_dec min a).
+        * exists min. splits; ss.
+          i. des; subst; eauto.
+        * exists a. splits; ss.
+          i. des; subst; try refl.
+          exploit MIN; eauto. i.
+          etrans; eauto. econs. ss.
+      + esplits; eauto. i. inv IN; eauto. ss.
+  Qed.
+
+  Lemma min_exists P cell:
+    (<<NONE: forall from to msg
+                    (GET: get to cell = Some (from, msg)),
+        ~ P to>>) \/
+    exists from_min to_min msg_min,
+      (<<GET: get to_min cell = Some (from_min, msg_min)>>) /\
+      (<<SAT: P to_min>>) /\
+      (<<MIN: forall from to msg
+                     (GET: get to cell = Some (from, msg))
+                     (SAT: P to),
+          Time.le to_min to>>).
+  Proof.
+    specialize (finite cell). i. des.
+    specialize (min_exists_aux
+                  (fun ts => P ts /\
+                             exists from msg,
+                               get ts cell = Some (from, msg))
+                  dom).
+    i. des.
+    - left. ii. exploit H; eauto. i.
+      exploit NONE; eauto.
+    - right. esplits; eauto. i.
+      exploit H; eauto.
+  Qed.
+
+
   (* next & previous greater timestamp *)
 
-  Fixpoint next (t: Time.t) (l: list Time.t) (res: option Time.t): option Time.t :=
-    match l with
-    | [] => res
-    | hd :: tl =>
-      if (Time.le_lt_dec hd t)
-      then next t tl res
-      else
-        match res with
-        | Some res =>
-          if (Time.le_lt_dec res hd)
-          then next t tl (Some res)
-          else next t tl (Some hd)
-        | None => next t tl (Some hd)
-        end
-    end.
+  (* Fixpoint next (t: Time.t) (l: list Time.t) (res: option Time.t): option Time.t := *)
+  (*   match l with *)
+  (*   | [] => res *)
+  (*   | hd :: tl => *)
+  (*     if (Time.le_lt_dec hd t) *)
+  (*     then next t tl res *)
+  (*     else *)
+  (*       match res with *)
+  (*       | Some res => *)
+  (*         if (Time.le_lt_dec res hd) *)
+  (*         then next t tl (Some res) *)
+  (*         else next t tl (Some hd) *)
+  (*       | None => next t tl (Some hd) *)
+  (*       end *)
+  (*   end. *)
 
-  Lemma next_le
-        t tnext init l
-        (NEXT: next t l (Some init) = Some tnext):
-    Time.le tnext init.
-  Proof.
-    revert init NEXT. induction l; ss; i.
-    - inv NEXT. refl.
-    - revert NEXT. repeat (condtac; ss); i.
-      + exploit IHl; try exact NEXT. i. auto.
-      + exploit IHl; try exact NEXT. i. auto.
-      + exploit IHl; try exact NEXT. i.
-        econs. eapply TimeFacts.le_lt_lt; eauto.
-  Qed.
+  (* Lemma next_le *)
+  (*       t tnext init l *)
+  (*       (NEXT: next t l (Some init) = Some tnext): *)
+  (*   Time.le tnext init. *)
+  (* Proof. *)
+  (*   revert init NEXT. induction l; ss; i. *)
+  (*   - inv NEXT. refl. *)
+  (*   - revert NEXT. repeat (condtac; ss); i. *)
+  (*     + exploit IHl; try exact NEXT. i. auto. *)
+  (*     + exploit IHl; try exact NEXT. i. auto. *)
+  (*     + exploit IHl; try exact NEXT. i. *)
+  (*       econs. eapply TimeFacts.le_lt_lt; eauto. *)
+  (* Qed. *)
 
-  Lemma next_spec_Some_aux
-        t tnext init l
-        (NEXT: next t l init = Some tnext):
-    (init = Some tnext /\
-     forall ts (TS1: Time.lt t ts) (TS2: Time.lt ts tnext),
-       ~ List.In ts l) \/
-    (List.In tnext l /\
-     Time.lt t tnext /\
-     forall ts (TS1: Time.lt t ts) (TS2: Time.lt ts tnext),
-       ~ List.In ts l).
-  Proof.
-    revert t tnext init NEXT. induction l; ss; i.
-    { left. ss. }
-    revert NEXT. condtac; ss; i.
-    - exploit IHl; eauto. intros x. des.
-      + subst. left. split; auto. ii. des.
-        * subst. timetac.
-        * eapply x0; eauto.
-      + right. splits; eauto. ii. des.
-        * subst. timetac.
-        * eapply x1; eauto.
-    - destruct init0.
-      + revert NEXT. condtac; ss; i.
-        * exploit IHl; eauto. intros x. des.
-          { inv x. left. split; auto. ii. des.
-            - subst. timetac.
-            - eapply x0; eauto. }
-          { right. splits; eauto. ii. des.
-            - subst. exploit next_le; eauto. i.
-              rewrite l1 in x3. timetac.
-            - eapply x1; eauto. }
-        * exploit IHl; eauto. intros x. des.
-          { inv x. right. splits; eauto. ii. des.
-            - subst. timetac.
-            - eapply x0; eauto. }
-          { right. splits; eauto. ii. des.
-            - subst. exploit next_le; eauto. i. timetac.
-            - eapply x1; eauto. }
-      + right. exploit IHl; eauto. intros x. des.
-        * inv x. esplits; eauto. ii. des.
-          { subst. timetac. }
-          { eapply x0; eauto. }
-        * esplits; eauto. ii. des.
-          { subst. exploit next_le; eauto. i. timetac. }
-          { eapply x1; eauto. }
-  Qed.
+  (* Lemma next_spec_Some_aux *)
+  (*       t tnext init l *)
+  (*       (NEXT: next t l init = Some tnext): *)
+  (*   (init = Some tnext /\ *)
+  (*    forall ts (TS1: Time.lt t ts) (TS2: Time.lt ts tnext), *)
+  (*      ~ List.In ts l) \/ *)
+  (*   (List.In tnext l /\ *)
+  (*    Time.lt t tnext /\ *)
+  (*    forall ts (TS1: Time.lt t ts) (TS2: Time.lt ts tnext), *)
+  (*      ~ List.In ts l). *)
+  (* Proof. *)
+  (*   revert t tnext init NEXT. induction l; ss; i. *)
+  (*   { left. ss. } *)
+  (*   revert NEXT. condtac; ss; i. *)
+  (*   - exploit IHl; eauto. intros x. des. *)
+  (*     + subst. left. split; auto. ii. des. *)
+  (*       * subst. timetac. *)
+  (*       * eapply x0; eauto. *)
+  (*     + right. splits; eauto. ii. des. *)
+  (*       * subst. timetac. *)
+  (*       * eapply x1; eauto. *)
+  (*   - destruct init0. *)
+  (*     + revert NEXT. condtac; ss; i. *)
+  (*       * exploit IHl; eauto. intros x. des. *)
+  (*         { inv x. left. split; auto. ii. des. *)
+  (*           - subst. timetac. *)
+  (*           - eapply x0; eauto. } *)
+  (*         { right. splits; eauto. ii. des. *)
+  (*           - subst. exploit next_le; eauto. i. *)
+  (*             rewrite l1 in x3. timetac. *)
+  (*           - eapply x1; eauto. } *)
+  (*       * exploit IHl; eauto. intros x. des. *)
+  (*         { inv x. right. splits; eauto. ii. des. *)
+  (*           - subst. timetac. *)
+  (*           - eapply x0; eauto. } *)
+  (*         { right. splits; eauto. ii. des. *)
+  (*           - subst. exploit next_le; eauto. i. timetac. *)
+  (*           - eapply x1; eauto. } *)
+  (*     + right. exploit IHl; eauto. intros x. des. *)
+  (*       * inv x. esplits; eauto. ii. des. *)
+  (*         { subst. timetac. } *)
+  (*         { eapply x0; eauto. } *)
+  (*       * esplits; eauto. ii. des. *)
+  (*         { subst. exploit next_le; eauto. i. timetac. } *)
+  (*         { eapply x1; eauto. } *)
+  (* Qed. *)
 
-  Lemma next_spec_Some
-        t tnext l
-        (NEXT: next t l None = Some tnext):
-    List.In tnext l /\
-    Time.lt t tnext /\
-    forall ts (TS1: Time.lt t ts) (TS2: Time.lt ts tnext),
-      ~ List.In ts l.
-  Proof.
-    exploit next_spec_Some_aux; eauto. i.
-    des; try congr; eauto.
-  Qed.
+  (* Lemma next_spec_Some *)
+  (*       t tnext l *)
+  (*       (NEXT: next t l None = Some tnext): *)
+  (*   List.In tnext l /\ *)
+  (*   Time.lt t tnext /\ *)
+  (*   forall ts (TS1: Time.lt t ts) (TS2: Time.lt ts tnext), *)
+  (*     ~ List.In ts l. *)
+  (* Proof. *)
+  (*   exploit next_spec_Some_aux; eauto. i. *)
+  (*   des; try congr; eauto. *)
+  (* Qed. *)
 
-  Lemma next_spec_None_aux
-        t init l:
-    next t l (Some init) <> None.
-  Proof.
-    revert t init. induction l; ss; i.
-    repeat condtac; ss; eauto.
-  Qed.
+  (* Lemma next_spec_None_aux *)
+  (*       t init l: *)
+  (*   next t l (Some init) <> None. *)
+  (* Proof. *)
+  (*   revert t init. induction l; ss; i. *)
+  (*   repeat condtac; ss; eauto. *)
+  (* Qed. *)
 
-  Lemma next_spec_None
-        t l
-        (NEXT: next t l None = None):
-    forall ts (IN: List.In ts l),
-      Time.le ts t.
-  Proof.
-    revert t NEXT. induction l; ss; i. des.
-    - subst. revert NEXT. condtac; ss; i.
-      specialize (next_spec_None_aux t0 ts l). congr.
-    - revert NEXT. condtac; ss; i.
-      + exploit IHl; eauto.
-      + specialize (next_spec_None_aux t0 a l). congr.
-  Qed.
+  (* Lemma next_spec_None *)
+  (*       t l *)
+  (*       (NEXT: next t l None = None): *)
+  (*   forall ts (IN: List.In ts l), *)
+  (*     Time.le ts t. *)
+  (* Proof. *)
+  (*   revert t NEXT. induction l; ss; i. des. *)
+  (*   - subst. revert NEXT. condtac; ss; i. *)
+  (*     specialize (next_spec_None_aux t0 ts l). congr. *)
+  (*   - revert NEXT. condtac; ss; i. *)
+  (*     + exploit IHl; eauto. *)
+  (*     + specialize (next_spec_None_aux t0 a l). congr. *)
+  (* Qed. *)
 
   Lemma next_exists
         cell f t m ts
@@ -614,135 +717,126 @@ Module Cell.
       forall ts' (TS1: Time.lt ts ts') (TS2: Time.lt ts' to),
         get ts' cell = None.
   Proof.
-    destruct cell. unfold get in *. ss.
-    destruct (next ts (List.map (fun x => fst x) (DOMap.elements raw0)) None) eqn:NEXT.
-    - exploit next_spec_Some; eauto. i. des.
-      exploit in_prod_inv; eauto. i. des. destruct b.
-      exploit DOMap.elements_complete; eauto. i.
-      esplits; try exact x4; eauto. i.
-      destruct (DOMap.find ts' raw0) as [[]|] eqn:GET; ss.
-      exploit DOMap.elements_correct; try exact GET. i.
-      exploit in_prod; try exact x5. i.
-      exploit x2; eauto. ss.
-    - exploit (@max_ts_spec t f m (Cell.mk WF0)); ss. i. des.
-      unfold get in *. ss.
-      exploit DOMap.elements_correct; try exact GET. i.
-      exploit in_prod; try exact x0. i.
-      exploit next_spec_None; eauto. i. timetac.
+    specialize (min_exists (fun ts' => Time.lt ts ts') cell). i. des.
+    - exploit max_ts_spec; eauto. i. des.
+      exploit NONE; eauto. ss.
+    - esplits; try exact GET; eauto. i.
+      destruct (get ts' cell) as [[]|] eqn:GET'; ss.
+      exploit MIN; try exact GET'; ss. i. timetac.
   Qed.
 
-  Fixpoint prev (t: Time.t) (l: list Time.t) (res: option Time.t): option Time.t :=
-    match l with
-    | [] => res
-    | hd :: tl =>
-      if (Time.le_lt_dec t hd)
-      then prev t tl res
-      else
-        match res with
-        | Some res =>
-          if (Time.le_lt_dec hd res)
-          then prev t tl (Some res)
-          else prev t tl (Some hd)
-        | None => prev t tl (Some hd)
-        end
-    end.
+  (* Fixpoint prev (t: Time.t) (l: list Time.t) (res: option Time.t): option Time.t := *)
+  (*   match l with *)
+  (*   | [] => res *)
+  (*   | hd :: tl => *)
+  (*     if (Time.le_lt_dec t hd) *)
+  (*     then prev t tl res *)
+  (*     else *)
+  (*       match res with *)
+  (*       | Some res => *)
+  (*         if (Time.le_lt_dec hd res) *)
+  (*         then prev t tl (Some res) *)
+  (*         else prev t tl (Some hd) *)
+  (*       | None => prev t tl (Some hd) *)
+  (*       end *)
+  (*   end. *)
 
-  Lemma prev_le
-        t tprev init l
-        (PREV: prev t l (Some init) = Some tprev):
-    Time.le init tprev.
-  Proof.
-    revert init PREV. induction l; ss; i.
-    - inv PREV. refl.
-    - revert PREV. repeat (condtac; ss); i.
-      + exploit IHl; try exact PREV. i. auto.
-      + exploit IHl; try exact PREV. i. auto.
-      + exploit IHl; try exact PREV. i.
-        econs. eapply TimeFacts.lt_le_lt; eauto.
-  Qed.
+  (* Lemma prev_le *)
+  (*       t tprev init l *)
+  (*       (PREV: prev t l (Some init) = Some tprev): *)
+  (*   Time.le init tprev. *)
+  (* Proof. *)
+  (*   revert init PREV. induction l; ss; i. *)
+  (*   - inv PREV. refl. *)
+  (*   - revert PREV. repeat (condtac; ss); i. *)
+  (*     + exploit IHl; try exact PREV. i. auto. *)
+  (*     + exploit IHl; try exact PREV. i. auto. *)
+  (*     + exploit IHl; try exact PREV. i. *)
+  (*       econs. eapply TimeFacts.lt_le_lt; eauto. *)
+  (* Qed. *)
 
-  Lemma prev_spec_Some_aux
-        t tprev init l
-        (PREV: prev t l init = Some tprev):
-    (init = Some tprev /\
-     forall ts (TS1: Time.lt tprev ts) (TS2: Time.lt ts t),
-       ~ List.In ts l) \/
-    (List.In tprev l /\
-     Time.lt tprev t /\
-     forall ts (TS1: Time.lt tprev ts) (TS2: Time.lt ts t),
-       ~ List.In ts l).
-  Proof.
-    revert t tprev init PREV. induction l; ss; i.
-    { left. ss. }
-    revert PREV. condtac; ss; i.
-    - exploit IHl; eauto. intros x. des.
-      + subst. left. split; auto. ii. des.
-        * subst. timetac.
-        * eapply x0; eauto.
-      + right. splits; eauto. ii. des.
-        * subst. timetac.
-        * eapply x1; eauto.
-    - destruct init0.
-      + revert PREV. condtac; ss; i.
-        * exploit IHl; eauto. intros x. des.
-          { inv x. left. split; auto. ii. des.
-            - subst. timetac.
-            - eapply x0; eauto. }
-          { right. splits; eauto. ii. des.
-            - subst. exploit prev_le; eauto. i.
-              eapply Time.lt_strorder.
-              eapply TimeFacts.le_lt_lt; try exact TS1.
-              etrans; eauto.
-            - eapply x1; eauto. }
-        * exploit IHl; eauto. intros x. des.
-          { inv x. right. splits; eauto. ii. des.
-            - subst. timetac.
-            - eapply x0; eauto. }
-          { right. splits; eauto. ii. des.
-            - subst. exploit prev_le; eauto. i. timetac.
-            - eapply x1; eauto. }
-      + right. exploit IHl; eauto. intros x. des.
-        * inv x. esplits; eauto. ii. des.
-          { subst. timetac. }
-          { eapply x0; eauto. }
-        * esplits; eauto. ii. des.
-          { subst. exploit prev_le; eauto. i. timetac. }
-          { eapply x1; eauto. }
-  Qed.
+  (* Lemma prev_spec_Some_aux *)
+  (*       t tprev init l *)
+  (*       (PREV: prev t l init = Some tprev): *)
+  (*   (init = Some tprev /\ *)
+  (*    forall ts (TS1: Time.lt tprev ts) (TS2: Time.lt ts t), *)
+  (*      ~ List.In ts l) \/ *)
+  (*   (List.In tprev l /\ *)
+  (*    Time.lt tprev t /\ *)
+  (*    forall ts (TS1: Time.lt tprev ts) (TS2: Time.lt ts t), *)
+  (*      ~ List.In ts l). *)
+  (* Proof. *)
+  (*   revert t tprev init PREV. induction l; ss; i. *)
+  (*   { left. ss. } *)
+  (*   revert PREV. condtac; ss; i. *)
+  (*   - exploit IHl; eauto. intros x. des. *)
+  (*     + subst. left. split; auto. ii. des. *)
+  (*       * subst. timetac. *)
+  (*       * eapply x0; eauto. *)
+  (*     + right. splits; eauto. ii. des. *)
+  (*       * subst. timetac. *)
+  (*       * eapply x1; eauto. *)
+  (*   - destruct init0. *)
+  (*     + revert PREV. condtac; ss; i. *)
+  (*       * exploit IHl; eauto. intros x. des. *)
+  (*         { inv x. left. split; auto. ii. des. *)
+  (*           - subst. timetac. *)
+  (*           - eapply x0; eauto. } *)
+  (*         { right. splits; eauto. ii. des. *)
+  (*           - subst. exploit prev_le; eauto. i. *)
+  (*             eapply Time.lt_strorder. *)
+  (*             eapply TimeFacts.le_lt_lt; try exact TS1. *)
+  (*             etrans; eauto. *)
+  (*           - eapply x1; eauto. } *)
+  (*       * exploit IHl; eauto. intros x. des. *)
+  (*         { inv x. right. splits; eauto. ii. des. *)
+  (*           - subst. timetac. *)
+  (*           - eapply x0; eauto. } *)
+  (*         { right. splits; eauto. ii. des. *)
+  (*           - subst. exploit prev_le; eauto. i. timetac. *)
+  (*           - eapply x1; eauto. } *)
+  (*     + right. exploit IHl; eauto. intros x. des. *)
+  (*       * inv x. esplits; eauto. ii. des. *)
+  (*         { subst. timetac. } *)
+  (*         { eapply x0; eauto. } *)
+  (*       * esplits; eauto. ii. des. *)
+  (*         { subst. exploit prev_le; eauto. i. timetac. } *)
+  (*         { eapply x1; eauto. } *)
+  (* Qed. *)
 
-  Lemma prev_spec_Some
-        t tprev l
-        (PREV: prev t l None = Some tprev):
-    List.In tprev l /\
-    Time.lt tprev t /\
-    forall ts (TS1: Time.lt tprev ts) (TS2: Time.lt ts t),
-      ~ List.In ts l.
-  Proof.
-    exploit prev_spec_Some_aux; eauto. i.
-    des; try congr; eauto.
-  Qed.
+  (* Lemma prev_spec_Some *)
+  (*       t tprev l *)
+  (*       (PREV: prev t l None = Some tprev): *)
+  (*   List.In tprev l /\ *)
+  (*   Time.lt tprev t /\ *)
+  (*   forall ts (TS1: Time.lt tprev ts) (TS2: Time.lt ts t), *)
+  (*     ~ List.In ts l. *)
+  (* Proof. *)
+  (*   exploit prev_spec_Some_aux; eauto. i. *)
+  (*   des; try congr; eauto. *)
+  (* Qed. *)
 
-  Lemma prev_spec_None_aux
-        t init l:
-    prev t l (Some init) <> None.
-  Proof.
-    revert t init. induction l; ss; i.
-    repeat condtac; ss; eauto.
-  Qed.
+  (* Lemma prev_spec_None_aux *)
+  (*       t init l: *)
+  (*   prev t l (Some init) <> None. *)
+  (* Proof. *)
+  (*   revert t init. induction l; ss; i. *)
+  (*   repeat condtac; ss; eauto. *)
+  (* Qed. *)
 
-  Lemma prev_spec_None
-        t l
-        (PREV: prev t l None = None):
-    forall ts (IN: List.In ts l),
-      Time.le t ts.
-  Proof.
-    revert t PREV. induction l; ss; i. des.
-    - subst. revert PREV. condtac; ss; i.
-      specialize (prev_spec_None_aux t0 ts l). congr.
-    - revert PREV. condtac; ss; i.
-      + exploit IHl; eauto.
-      + specialize (prev_spec_None_aux t0 a l). congr.
-  Qed.
+  (* Lemma prev_spec_None *)
+  (*       t l *)
+  (*       (PREV: prev t l None = None): *)
+  (*   forall ts (IN: List.In ts l), *)
+  (*     Time.le t ts. *)
+  (* Proof. *)
+  (*   revert t PREV. induction l; ss; i. des. *)
+  (*   - subst. revert PREV. condtac; ss; i. *)
+  (*     specialize (prev_spec_None_aux t0 ts l). congr. *)
+  (*   - revert PREV. condtac; ss; i. *)
+  (*     + exploit IHl; eauto. *)
+  (*     + specialize (prev_spec_None_aux t0 a l). congr. *)
+  (* Qed. *)
 
   Lemma prev_exists
         cell f t m ts
@@ -754,19 +848,24 @@ Module Cell.
       forall ts' (TS1: Time.lt to ts') (TS2: Time.lt ts' ts),
         get ts' cell = None.
   Proof.
-    destruct cell. unfold get in *. ss.
-    destruct (prev ts (List.map (fun x => fst x) (DOMap.elements raw0)) None) eqn:PREV.
-    - exploit prev_spec_Some; eauto. i. des.
-      exploit in_prod_inv; eauto. i. des. destruct b.
-      exploit DOMap.elements_complete; eauto. i.
-      esplits; try exact x4; eauto. i.
-      destruct (DOMap.find ts' raw0) as [[]|] eqn:GET; ss.
-      exploit DOMap.elements_correct; try exact GET. i.
-      exploit in_prod; try exact x5. i.
-      exploit x2; eauto. ss.
-    - exploit DOMap.elements_correct; try exact INHABITED. i.
-      exploit in_prod; try exact x0. i.
-      exploit prev_spec_None; eauto. i. timetac.
+    specialize (max_exists (fun ts' => Time.lt ts' ts) cell). i. des.
+    - exploit NONE; eauto. ss.
+    - esplits; try exact GET; eauto. i.
+      destruct (get ts' cell) as [[]|] eqn:GET'; ss.
+      exploit MAX; try exact GET'; ss. i. timetac.
+    (* destruct cell. unfold get in *. ss. *)
+    (* destruct (prev ts (List.map (fun x => fst x) (DOMap.elements raw0)) None) eqn:PREV. *)
+    (* - exploit prev_spec_Some; eauto. i. des. *)
+    (*   exploit in_prod_inv; eauto. i. des. destruct b. *)
+    (*   exploit DOMap.elements_complete; eauto. i. *)
+    (*   esplits; try exact x4; eauto. i. *)
+    (*   destruct (DOMap.find ts' raw0) as [[]|] eqn:GET; ss. *)
+    (*   exploit DOMap.elements_correct; try exact GET. i. *)
+    (*   exploit in_prod; try exact x5. i. *)
+    (*   exploit x2; eauto. ss. *)
+    (* - exploit DOMap.elements_correct; try exact INHABITED. i. *)
+    (*   exploit in_prod; try exact x0. i. *)
+    (*   exploit prev_spec_None; eauto. i. timetac. *)
   Qed.
 
 
