src/model/PFConfiguration.v
@@ -31,7 +31,8 @@ Module PFConfiguration.
         (TID: IdentMap.find tid (Configuration.threads c1) = Some (existT _ lang st1, lc1))
         (STEP: Thread.step e
                  (Thread.mk _ st1 lc1 (Configuration.global c1))
-                 (Thread.mk _ st2 lc2 gl2)):
+                 (Thread.mk _ st2 lc2 gl2))
+        (EVENT: ThreadEvent.is_program e):
       estep e tid
             c1
             (Configuration.mk (IdentMap.add tid (existT _ _ st2, lc2) (Configuration.threads c1)) gl2)
@@ -209,7 +210,8 @@ Module PFConfiguration.
           c1 tid lang st1 lc1
           e th2
           (FIND: IdentMap.find tid (Configuration.threads c1) = Some (existT _ lang st1, lc1))
-          (STEP: Thread.step e (Thread.mk _ st1 lc1 (Configuration.global c1)) th2):
+          (STEP: Thread.step e (Thread.mk _ st1 lc1 (Configuration.global c1)) th2)
+          (EVENT: ThreadEvent.is_program e):
       step (get_machine_event e) tid
            c1
            (Configuration.mk
@@ -224,7 +226,8 @@ Module PFConfiguration.
         c1 tid lang st1 lc1
         e th2
         (FIND: IdentMap.find tid (Configuration.threads c1) = Some (existT _ lang st1, lc1))
-        (STEP: Thread.opt_step e (Thread.mk _ st1 lc1 (Configuration.global c1)) th2):
+        (STEP: Thread.opt_step e (Thread.mk _ st1 lc1 (Configuration.global c1)) th2)
+        (EVENT: ThreadEvent.is_program e):
     opt_step ThreadEvent.get_machine_event_pf
              (ThreadEvent.get_machine_event_pf e) tid
              c1
@@ -238,109 +241,109 @@ Module PFConfiguration.
     - econs 2. econs; eauto.
   Qed.
 
-  Lemma rtc_program_step_rtc_step
-        c1 tid lang st1 lc1
-        th2
-        (FIND: IdentMap.find tid (Configuration.threads c1) = Some (existT _ lang st1, lc1))
-        (STEPS: rtc (pstep (@Thread.step lang) (ThreadEvent.is_silent /1\ThreadEvent.is_program))
-                    (Thread.mk _ st1 lc1 (Configuration.global c1)) th2):
-    (<<STEPS: rtc (tau_step ThreadEvent.get_machine_event_pf)
-                  c1
-                  (Configuration.mk
-                     (IdentMap.add tid (existT _ _ (Thread.state th2), Thread.local th2) (Configuration.threads c1))
-                     (Thread.global th2))>>) \/
-    exists c2 c3,
-      (<<STEPS: rtc (tau_step ThreadEvent.get_machine_event_pf) c1 c2>>) /\
-      (<<STEP: step ThreadEvent.get_machine_event_pf MachineEvent.failure tid c2 c3>>).
-  Proof.
-    destruct c1 as [ths1 gl1]. ss.
-    remember (Thread.mk _ st1 lc1 gl1) as th1.
-    replace st1 with (Thread.state th1) in FIND by (subst; ss).
-    replace lc1 with (Thread.local th1) in FIND by (subst; ss).
-    replace gl1 with (Thread.global th1) by (subst; ss).
-    clear gl1 st1 lc1 Heqth1. revert ths1 FIND.
-    induction STEPS; i; subst; ss.
-    { left. rewrite IdentMap.gsident; ss. auto. }
-    destruct x, y. inv H. ss.
-    destruct (ThreadEvent.get_machine_event_pf e) eqn: PF_EVENT; cycle 1.
-    { des. destruct e; ss. }
-    { right. esplits; [refl|].
-      rewrite <- PF_EVENT. econs. econs; eauto.
-    }
-    exploit (@program_step_step
-               ThreadEvent.get_machine_event_pf (Configuration.mk ths1 global)); eauto. s. i.
-    exploit (IHSTEPS
-               (IdentMap.add tid (existT (Language.state (E:=ProgramEvent.t)) lang state0, local0) ths1));
-      try apply IdentMap.gss.
-    i. des.
-    - rewrite IdentMap.add_add_eq in *.
-      left. econs 2; eauto. econs. rewrite <- PF_EVENT. eauto.
-    - right. esplits; try exact STEP0.
-      econs 2; eauto. econs. rewrite <- PF_EVENT. eauto.
-  Qed.
+  (* Lemma rtc_program_step_rtc_step *)
+  (*       c1 tid lang st1 lc1 *)
+  (*       th2 *)
+  (*       (FIND: IdentMap.find tid (Configuration.threads c1) = Some (existT _ lang st1, lc1)) *)
+  (*       (STEPS: rtc (pstep (@Thread.step lang) (ThreadEvent.is_silent /1\ThreadEvent.is_program)) *)
+  (*                   (Thread.mk _ st1 lc1 (Configuration.global c1)) th2): *)
+  (*   (<<STEPS: rtc (tau_step ThreadEvent.get_machine_event_pf) *)
+  (*                 c1 *)
+  (*                 (Configuration.mk *)
+  (*                    (IdentMap.add tid (existT _ _ (Thread.state th2), Thread.local th2) (Configuration.threads c1)) *)
+  (*                    (Thread.global th2))>>) \/ *)
+  (*   exists c2 c3, *)
+  (*     (<<STEPS: rtc (tau_step ThreadEvent.get_machine_event_pf) c1 c2>>) /\ *)
+  (*     (<<STEP: step ThreadEvent.get_machine_event_pf MachineEvent.failure tid c2 c3>>). *)
+  (* Proof. *)
+  (*   destruct c1 as [ths1 gl1]. ss. *)
+  (*   remember (Thread.mk _ st1 lc1 gl1) as th1. *)
+  (*   replace st1 with (Thread.state th1) in FIND by (subst; ss). *)
+  (*   replace lc1 with (Thread.local th1) in FIND by (subst; ss). *)
+  (*   replace gl1 with (Thread.global th1) by (subst; ss). *)
+  (*   clear gl1 st1 lc1 Heqth1. revert ths1 FIND. *)
+  (*   induction STEPS; i; subst; ss. *)
+  (*   { left. rewrite IdentMap.gsident; ss. auto. } *)
+  (*   destruct x, y. inv H. ss. *)
+  (*   destruct (ThreadEvent.get_machine_event_pf e) eqn: PF_EVENT; cycle 1. *)
+  (*   { des. destruct e; ss. } *)
+  (*   { right. esplits; [refl|]. *)
+  (*     rewrite <- PF_EVENT. econs. econs; eauto. *)
+  (*   } *)
+  (*   exploit (@program_step_step *)
+  (*              ThreadEvent.get_machine_event_pf (Configuration.mk ths1 global)); eauto. s. i. *)
+  (*   exploit (IHSTEPS *)
+  (*              (IdentMap.add tid (existT (Language.state (E:=ProgramEvent.t)) lang state0, local0) ths1)); *)
+  (*     try apply IdentMap.gss. *)
+  (*   i. des. *)
+  (*   - rewrite IdentMap.add_add_eq in *. *)
+  (*     left. econs 2; eauto. econs. rewrite <- PF_EVENT. eauto. *)
+  (*   - right. esplits; try exact STEP0. *)
+  (*     econs 2; eauto. econs. rewrite <- PF_EVENT. eauto. *)
+  (* Qed. *)
 
-  Lemma plus_program_step_plus_step
-        c1 tid lang st1 lc1
-        e th2 th3
-        (FIND: IdentMap.find tid (Configuration.threads c1) = Some (existT _ lang st1, lc1))
-        (STEPS: rtc (pstep (@Thread.step lang) (ThreadEvent.is_silent /1\ ThreadEvent.is_program))
-                    (Thread.mk _ st1 lc1 (Configuration.global c1)) th2)
-        (STEP: Thread.step e th2 th3):
-    (exists c2,
-        (<<STEPS: rtc (tau_step ThreadEvent.get_machine_event_pf) c1 c2>>) /\
-        (<<STEP: step ThreadEvent.get_machine_event_pf (ThreadEvent.get_machine_event_pf e) tid
-                      c2
-                      (Configuration.mk
-                         (IdentMap.add tid (existT _ _ (Thread.state th3), Thread.local th3) (Configuration.threads c1))
-                         (Thread.global th3))>>) /\
-        (<<EVENT: ThreadEvent.get_machine_event_pf e <> MachineEvent.failure>>)) \/
-    (exists c2 c3,
-        (<<STEPS: rtc (tau_step ThreadEvent.get_machine_event_pf) c1 c2>>) /\
-        (<<STEP: step ThreadEvent.get_machine_event_pf MachineEvent.failure tid c2 c3>>)).
-  Proof.
-    exploit rtc_program_step_rtc_step; eauto. i. des; eauto.
-    destruct th2. ss.
-    exploit (@program_step_step
-               ThreadEvent.get_machine_event_pf
-               (Configuration.mk
-                  (IdentMap.add tid (existT _ lang state, local) (Configuration.threads c1))
-                  global)); s; try apply IdentMap.gss; eauto.
-    rewrite IdentMap.add_add_eq.
-    i. destruct (classic (ThreadEvent.get_machine_event_pf e = MachineEvent.failure)).
-    - right. rewrite H in *. esplits; eauto.
-    - left. esplits; eauto.
-  Qed.
+  (* Lemma plus_program_step_plus_step *)
+  (*       c1 tid lang st1 lc1 *)
+  (*       e th2 th3 *)
+  (*       (FIND: IdentMap.find tid (Configuration.threads c1) = Some (existT _ lang st1, lc1)) *)
+  (*       (STEPS: rtc (pstep (@Thread.step lang) (ThreadEvent.is_silent /1\ ThreadEvent.is_program)) *)
+  (*                   (Thread.mk _ st1 lc1 (Configuration.global c1)) th2) *)
+  (*       (STEP: Thread.step e th2 th3): *)
+  (*   (exists c2, *)
+  (*       (<<STEPS: rtc (tau_step ThreadEvent.get_machine_event_pf) c1 c2>>) /\ *)
+  (*       (<<STEP: step ThreadEvent.get_machine_event_pf (ThreadEvent.get_machine_event_pf e) tid *)
+  (*                     c2 *)
+  (*                     (Configuration.mk *)
+  (*                        (IdentMap.add tid (existT _ _ (Thread.state th3), Thread.local th3) (Configuration.threads c1)) *)
+  (*                        (Thread.global th3))>>) /\ *)
+  (*       (<<EVENT: ThreadEvent.get_machine_event_pf e <> MachineEvent.failure>>)) \/ *)
+  (*   (exists c2 c3, *)
+  (*       (<<STEPS: rtc (tau_step ThreadEvent.get_machine_event_pf) c1 c2>>) /\ *)
+  (*       (<<STEP: step ThreadEvent.get_machine_event_pf MachineEvent.failure tid c2 c3>>)). *)
+  (* Proof. *)
+  (*   exploit rtc_program_step_rtc_step; eauto. i. des; eauto. *)
+  (*   destruct th2. ss. *)
+  (*   exploit (@program_step_step *)
+  (*              ThreadEvent.get_machine_event_pf *)
+  (*              (Configuration.mk *)
+  (*                 (IdentMap.add tid (existT _ lang state, local) (Configuration.threads c1)) *)
+  (*                 global)); s; try apply IdentMap.gss; eauto. *)
+  (*   rewrite IdentMap.add_add_eq. *)
+  (*   i. destruct (classic (ThreadEvent.get_machine_event_pf e = MachineEvent.failure)). *)
+  (*   - right. rewrite H in *. esplits; eauto. *)
+  (*   - left. esplits; eauto. *)
+  (* Qed. *)
 
-  Lemma opt_plus_program_step_opt_plus_step
-        c1 tid lang st1 lc1
-        e th2 th3
-        (FIND: IdentMap.find tid (Configuration.threads c1) = Some (existT _ lang st1, lc1))
-        (STEPS: rtc (pstep (@Thread.step lang) (ThreadEvent.is_silent /1\ ThreadEvent.is_program))
-                    (Thread.mk _ st1 lc1 (Configuration.global c1)) th2)
-        (STEP: Thread.opt_step e th2 th3):
-    (exists c2,
-        (<<STEPS: rtc (tau_step ThreadEvent.get_machine_event_pf) c1 c2>>) /\
-        (<<STEP: opt_step ThreadEvent.get_machine_event_pf (ThreadEvent.get_machine_event_pf e) tid
-                          c2
-                          (Configuration.mk
-                             (IdentMap.add tid (existT _ _ (Thread.state th3), Thread.local th3) (Configuration.threads c1))
-                             (Thread.global th3))>>) /\
-        (<<EVENT: ThreadEvent.get_machine_event_pf e <> MachineEvent.failure>>)) \/
-    (exists c2 c3,
-        (<<STEPS: rtc (tau_step ThreadEvent.get_machine_event_pf) c1 c2>>) /\
-        (<<STEP: step ThreadEvent.get_machine_event_pf MachineEvent.failure tid c2 c3>>)).
-  Proof.
-    exploit rtc_program_step_rtc_step; eauto. i. des; eauto.
-    destruct th2. ss.
-    exploit (@opt_program_step_opt_step
-               (Configuration.mk
-                  (IdentMap.add tid (existT _ lang state, local) (Configuration.threads c1))
-                  global)); s; try apply IdentMap.gss; eauto.
-    rewrite IdentMap.add_add_eq.
-    i. destruct (classic (ThreadEvent.get_machine_event_pf e = MachineEvent.failure)).
-    - right. rewrite H in *. inv x0. esplits; eauto.
-    - left. esplits; eauto.
-  Qed.
+  (* Lemma opt_plus_program_step_opt_plus_step *)
+  (*       c1 tid lang st1 lc1 *)
+  (*       e th2 th3 *)
+  (*       (FIND: IdentMap.find tid (Configuration.threads c1) = Some (existT _ lang st1, lc1)) *)
+  (*       (STEPS: rtc (pstep (@Thread.step lang) (ThreadEvent.is_silent /1\ ThreadEvent.is_program)) *)
+  (*                   (Thread.mk _ st1 lc1 (Configuration.global c1)) th2) *)
+  (*       (STEP: Thread.opt_step e th2 th3): *)
+  (*   (exists c2, *)
+  (*       (<<STEPS: rtc (tau_step ThreadEvent.get_machine_event_pf) c1 c2>>) /\ *)
+  (*       (<<STEP: opt_step ThreadEvent.get_machine_event_pf (ThreadEvent.get_machine_event_pf e) tid *)
+  (*                         c2 *)
+  (*                         (Configuration.mk *)
+  (*                            (IdentMap.add tid (existT _ _ (Thread.state th3), Thread.local th3) (Configuration.threads c1)) *)
+  (*                            (Thread.global th3))>>) /\ *)
+  (*       (<<EVENT: ThreadEvent.get_machine_event_pf e <> MachineEvent.failure>>)) \/ *)
+  (*   (exists c2 c3, *)
+  (*       (<<STEPS: rtc (tau_step ThreadEvent.get_machine_event_pf) c1 c2>>) /\ *)
+  (*       (<<STEP: step ThreadEvent.get_machine_event_pf MachineEvent.failure tid c2 c3>>)). *)
+  (* Proof. *)
+  (*   exploit rtc_program_step_rtc_step; eauto. i. des; eauto. *)
+  (*   destruct th2. ss. *)
+  (*   exploit (@opt_program_step_opt_step *)
+  (*              (Configuration.mk *)
+  (*                 (IdentMap.add tid (existT _ lang state, local) (Configuration.threads c1)) *)
+  (*                 global)); s; try apply IdentMap.gss; eauto. *)
+  (*   rewrite IdentMap.add_add_eq. *)
+  (*   i. destruct (classic (ThreadEvent.get_machine_event_pf e = MachineEvent.failure)). *)
+  (*   - right. rewrite H in *. inv x0. esplits; eauto. *)
+  (*   - left. esplits; eauto. *)
+  (* Qed. *)
 End PFConfiguration.
 #[export] Hint Constructors PFConfiguration.step: core.
 #[export] Hint Constructors PFConfiguration.normal_step: core.
